A first attempt at removing the fuel.

theories/interpreter.v
@@ -30,6 +30,8 @@ Let executable_host := executable_host host_function.
 Variable host_instance : executable_host.
 
 Let host_event := host_event host_instance.
+Let host_apply : store_record -> host_function -> seq value -> host_event (option (store_record * result)) :=
+  @host_apply _ host_instance.
 
 (* TODO: See ITree/tutorial/Imp.v
 Context {eff : Type -> Type}.
@@ -85,10 +87,6 @@ Canonical Structure res_step_eqType := Eval hnf in EqType res_step res_step_eqMi
 Definition crash_error := RS_crash C_error.
 
 Definition depth := nat.
-
-(** As Coq programs have to terminate, but Wasm programs don’t, we force termination
-  but relying on fuel. **)
-Definition fuel := nat.
 
 Definition config_tuple : Type := store_record * seq value * seq administrative_instruction.
 
@@ -164,388 +162,400 @@ Proof.
   - move=> >. by apply: ReflectF.
 Qed.
 
-Fixpoint run_step_with_fuel (fuel : fuel) (d : depth) (i : instance) (tt : config_tuple)
-    : itree host_event res_tuple :=
+(** An inductive for the [mrec] fixed-point combinator, expressing the signature of the
+   functions [run_step_base] and [run_one_step]. **)
+Inductive run_stepE : Type -> Type :=
+  | call_run_step_base :
+    depth -> instance -> config_tuple ->
+    run_stepE res_tuple
+  | call_run_one_step :
+    depth -> instance -> config_one_tuple_without_e -> administrative_instruction ->
+    run_stepE res_tuple
+  .
+
+Definition run_step_base (call : run_stepE ~> itree (run_stepE +' host_event))
+    (d : depth) (i : instance) (tt : config_tuple)
+  : itree (run_stepE +' host_event) res_tuple :=
   let: (s, vs, es) := tt in
-  match fuel with
-  | 0 => ret (s, vs, RS_crash C_exhaustion)
-  | fuel.+1 =>
-    let: (ves, es') := split_vals_e es in (** Framing out constants. **)
-    match es' with
-    | [::] => ret (s, vs, crash_error)
-    | e :: es'' =>
-      if e_is_trap e
-      then
-        if (es'' != [::]) || (ves != [::])
-        then ret (s, vs, RS_normal [::Trap])
-        else ret (s, vs, crash_error)
-      else
-        rosf <- run_one_step fuel d i (s, vs, (rev ves)) e ;;
-        let: (s', vs', r) := rosf in
-        if r is RS_normal res
-        then ret (s', vs', RS_normal (res ++ es''))
-        else ret (s', vs', r)
-    end
-  end
+  let: (ves, es') := split_vals_e es in (** Framing out constants. **)
+  match es' with
+  | [::] => ret (s, vs, crash_error)
+  | e :: es'' =>
+    if e_is_trap e
+    then
+      if (es'' != [::]) || (ves != [::])
+      then ret (s, vs, RS_normal [::Trap])
+      else ret (s, vs, crash_error)
+    else
+      '(s', vs', r) <- call _ (call_run_one_step d i (s, vs, (rev ves)) e) ;;
+      if r is RS_normal res
+      then ret (s', vs', RS_normal (res ++ es''))
+      else ret (s', vs', r)
+  end.
 
-with run_one_step (fuel : fuel) (d : depth) (i : instance) (tt : config_one_tuple_without_e) (e : administrative_instruction)
-    : itree host_event res_tuple :=
+Definition run_one_step (call : run_stepE ~> itree (run_stepE +' host_event))
+      (d : depth) (i : instance) (tt : config_one_tuple_without_e) (e : administrative_instruction)
+    : itree (run_stepE +' host_event) res_tuple :=
   let: (s, vs, ves) := tt in
-  match fuel with
-  | 0 => ret (s, vs, RS_crash C_exhaustion)
-  | fuel.+1 =>
-    match e with
+  match e with
 
-    (** unop **)
-    | Basic (Unop_i T_i32 iop) =>
-      if ves is ConstInt32 c :: ves' then
-        ret (s, vs, RS_normal (vs_to_es ((ConstInt32 (@app_unop_i i32t iop c)) :: ves')))
-      else ret (s, vs, crash_error)
-    | Basic (Unop_i T_i64 iop) =>
-      if ves is (ConstInt64 c) :: ves' then
-        ret (s, vs, RS_normal (vs_to_es ((ConstInt64 (@app_unop_i i64t iop c)) :: ves')))
-      else ret (s, vs, crash_error)
-    | Basic (Unop_i _ _) => ret (s, vs, crash_error)
-    | Basic (Unop_f T_f32 iop) =>
-      if ves is (ConstFloat32 c) :: ves' then
-        ret (s, vs, RS_normal (vs_to_es ((ConstFloat32 (@app_unop_f f32t iop c)) :: ves')))
-      else ret (s, vs, crash_error)
-    | Basic (Unop_f T_f64 iop) =>
-      if ves is (ConstFloat64 c) :: ves' then
-        ret (s, vs, RS_normal (vs_to_es ((ConstFloat64 (@app_unop_f f64t iop c)) :: ves')))
-      else ret (s, vs, crash_error)
-    | Basic (Unop_f _ _) => ret (s, vs, crash_error)
+  (** unop **)
+  | Basic (Unop_i T_i32 iop) =>
+    if ves is ConstInt32 c :: ves' then
+      ret (s, vs, RS_normal (vs_to_es ((ConstInt32 (@app_unop_i i32t iop c)) :: ves')))
+    else ret (s, vs, crash_error)
+  | Basic (Unop_i T_i64 iop) =>
+    if ves is (ConstInt64 c) :: ves' then
+      ret (s, vs, RS_normal (vs_to_es ((ConstInt64 (@app_unop_i i64t iop c)) :: ves')))
+    else ret (s, vs, crash_error)
+  | Basic (Unop_i _ _) => ret (s, vs, crash_error)
+  | Basic (Unop_f T_f32 iop) =>
+    if ves is (ConstFloat32 c) :: ves' then
+      ret (s, vs, RS_normal (vs_to_es ((ConstFloat32 (@app_unop_f f32t iop c)) :: ves')))
+    else ret (s, vs, crash_error)
+  | Basic (Unop_f T_f64 iop) =>
+    if ves is (ConstFloat64 c) :: ves' then
+      ret (s, vs, RS_normal (vs_to_es ((ConstFloat64 (@app_unop_f f64t iop c)) :: ves')))
+    else ret (s, vs, crash_error)
+  | Basic (Unop_f _ _) => ret (s, vs, crash_error)
 
-    (** binop **)
-    | Basic (Binop_i T_i32 iop) =>
-      if ves is (ConstInt32 c2) :: (ConstInt32 c1) :: ves' then
-        expect (@app_binop_i i32t iop c1 c2) (fun c =>
-            ret (s, vs, RS_normal (vs_to_es ((ConstInt32 c) :: ves'))))
-          (ret (s, vs, RS_normal ((vs_to_es ves') ++ [::Trap])))
-      else ret (s, vs, crash_error)
-    | Basic (Binop_i T_i64 iop) =>
-      if ves is (ConstInt64 c2) :: (ConstInt64 c1) :: ves' then
-        expect (@app_binop_i i64t iop c1 c2) (fun c =>
-            ret (s, vs, RS_normal (vs_to_es ((ConstInt64 c) :: ves'))))
-          (ret (s, vs, RS_normal ((vs_to_es ves') ++ [::Trap])))
-      else ret (s, vs, crash_error)
-    | Basic (Binop_i _ _) => ret (s, vs, crash_error)
-    | Basic (Binop_f T_f32 fop) =>
-      if ves is (ConstFloat32 c2) :: (ConstFloat32 c1) :: ves' then
-        expect (@app_binop_f f32t fop c1 c2) (fun c =>
-            ret (s, vs, RS_normal (vs_to_es ((ConstFloat32 c) :: ves'))))
-          (ret (s, vs, RS_normal ((vs_to_es ves') ++ [::Trap])))
-      else ret (s, vs, crash_error)
-    | Basic (Binop_f T_f64 fop) =>
-      if ves is (ConstFloat64 c2) :: (ConstFloat64 c1) :: ves' then
-        expect (@app_binop_f f64t fop c1 c2) (fun c =>
-             ret (s, vs, RS_normal (vs_to_es ((ConstFloat64 c) :: ves'))))
-          (ret (s, vs, RS_normal ((vs_to_es ves') ++ [::Trap])))
-      else ret (s, vs, crash_error)
-    | Basic (Binop_f _ _) => ret (s, vs, crash_error)
+  (** binop **)
+  | Basic (Binop_i T_i32 iop) =>
+    if ves is (ConstInt32 c2) :: (ConstInt32 c1) :: ves' then
+      expect (@app_binop_i i32t iop c1 c2) (fun c =>
+          ret (s, vs, RS_normal (vs_to_es ((ConstInt32 c) :: ves'))))
+        (ret (s, vs, RS_normal ((vs_to_es ves') ++ [::Trap])))
+    else ret (s, vs, crash_error)
+  | Basic (Binop_i T_i64 iop) =>
+    if ves is (ConstInt64 c2) :: (ConstInt64 c1) :: ves' then
+      expect (@app_binop_i i64t iop c1 c2) (fun c =>
+          ret (s, vs, RS_normal (vs_to_es ((ConstInt64 c) :: ves'))))
+        (ret (s, vs, RS_normal ((vs_to_es ves') ++ [::Trap])))
+    else ret (s, vs, crash_error)
+  | Basic (Binop_i _ _) => ret (s, vs, crash_error)
+  | Basic (Binop_f T_f32 fop) =>
+    if ves is (ConstFloat32 c2) :: (ConstFloat32 c1) :: ves' then
+      expect (@app_binop_f f32t fop c1 c2) (fun c =>
+          ret (s, vs, RS_normal (vs_to_es ((ConstFloat32 c) :: ves'))))
+        (ret (s, vs, RS_normal ((vs_to_es ves') ++ [::Trap])))
+    else ret (s, vs, crash_error)
+  | Basic (Binop_f T_f64 fop) =>
+    if ves is (ConstFloat64 c2) :: (ConstFloat64 c1) :: ves' then
+      expect (@app_binop_f f64t fop c1 c2) (fun c =>
+           ret (s, vs, RS_normal (vs_to_es ((ConstFloat64 c) :: ves'))))
+        (ret (s, vs, RS_normal ((vs_to_es ves') ++ [::Trap])))
+    else ret (s, vs, crash_error)
+  | Basic (Binop_f _ _) => ret (s, vs, crash_error)
 
-    (** testops **)
-    | Basic (Testop T_i32 testop) =>
-      if ves is (ConstInt32 c) :: ves' then
-        ret (s, vs, RS_normal (vs_to_es ((ConstInt32 (wasm_bool (@app_testop_i i32t testop c))) :: ves')))
-      else ret (s, vs, crash_error)
-    | Basic (Testop T_i64 testop) =>
-      if ves is (ConstInt64 c) :: ves' then
-        ret (s, vs, RS_normal (vs_to_es ((ConstInt32 (wasm_bool (@app_testop_i i64t testop c))) :: ves')))
-      else ret (s, vs, crash_error)
-    | Basic (Testop _ _) => ret (s, vs, crash_error)
+  (** testops **)
+  | Basic (Testop T_i32 testop) =>
+    if ves is (ConstInt32 c) :: ves' then
+      ret (s, vs, RS_normal (vs_to_es ((ConstInt32 (wasm_bool (@app_testop_i i32t testop c))) :: ves')))
+    else ret (s, vs, crash_error)
+  | Basic (Testop T_i64 testop) =>
+    if ves is (ConstInt64 c) :: ves' then
+      ret (s, vs, RS_normal (vs_to_es ((ConstInt32 (wasm_bool (@app_testop_i i64t testop c))) :: ves')))
+    else ret (s, vs, crash_error)
+  | Basic (Testop _ _) => ret (s, vs, crash_error)
 
-    (** relops **)
-    | Basic (Relop_i T_i32 iop) =>
-      if ves is (ConstInt32 c2) :: (ConstInt32 c1) :: ves' then
-        ret (s, vs, RS_normal (vs_to_es (ConstInt32 (wasm_bool (@app_relop_i i32t iop c1 c2)) :: ves')))
-      else ret (s, vs, crash_error)
-    | Basic (Relop_i T_i64 iop) =>
-      if ves is (ConstInt64 c2) :: (ConstInt64 c1) :: ves' then
-        ret (s, vs, RS_normal (vs_to_es (ConstInt32 (wasm_bool (@app_relop_i i64t iop c1 c2)) :: ves')))
-      else ret (s, vs, crash_error)
-    | Basic (Relop_i _ _) => ret (s, vs, crash_error)
-    | Basic (Relop_f T_f32 iop) =>
-      if ves is (ConstFloat32 c2) :: (ConstFloat32 c1) :: ves' then
-        ret (s, vs, RS_normal (vs_to_es (ConstInt32 (wasm_bool (@app_relop_f f32t iop c1 c2)) :: ves')))
-      else ret (s, vs, crash_error)
-    | Basic (Relop_f T_f64 iop) =>
-      if ves is (ConstFloat64 c2) :: (ConstFloat64 c1) :: ves' then
-        ret (s, vs, RS_normal (vs_to_es (ConstInt32 (wasm_bool (@app_relop_f f64t iop c1 c2)) :: ves')))
-      else ret (s, vs, crash_error)
-    | Basic (Relop_f _ _) => ret (s, vs, crash_error)
+  (** relops **)
+  | Basic (Relop_i T_i32 iop) =>
+    if ves is (ConstInt32 c2) :: (ConstInt32 c1) :: ves' then
+      ret (s, vs, RS_normal (vs_to_es (ConstInt32 (wasm_bool (@app_relop_i i32t iop c1 c2)) :: ves')))
+    else ret (s, vs, crash_error)
+  | Basic (Relop_i T_i64 iop) =>
+    if ves is (ConstInt64 c2) :: (ConstInt64 c1) :: ves' then
+      ret (s, vs, RS_normal (vs_to_es (ConstInt32 (wasm_bool (@app_relop_i i64t iop c1 c2)) :: ves')))
+    else ret (s, vs, crash_error)
+  | Basic (Relop_i _ _) => ret (s, vs, crash_error)
+  | Basic (Relop_f T_f32 iop) =>
+    if ves is (ConstFloat32 c2) :: (ConstFloat32 c1) :: ves' then
+      ret (s, vs, RS_normal (vs_to_es (ConstInt32 (wasm_bool (@app_relop_f f32t iop c1 c2)) :: ves')))
+    else ret (s, vs, crash_error)
+  | Basic (Relop_f T_f64 iop) =>
+    if ves is (ConstFloat64 c2) :: (ConstFloat64 c1) :: ves' then
+      ret (s, vs, RS_normal (vs_to_es (ConstInt32 (wasm_bool (@app_relop_f f64t iop c1 c2)) :: ves')))
+    else ret (s, vs, crash_error)
+  | Basic (Relop_f _ _) => ret (s, vs, crash_error)
 
-    (** convert and reinterpret **)
-    | Basic (Cvtop t2 Convert t1 sx) =>
-      if ves is v :: ves' then
-        if types_agree t1 v
-        then
-          expect (cvt t2 sx v) (fun v' =>
-               ret (s, vs, RS_normal (vs_to_es (v' :: ves'))))
-            (ret (s, vs, RS_normal ((vs_to_es ves') ++ [::Trap])))
-        else ret (s, vs, crash_error)
-      else ret (s, vs, crash_error)
-    | Basic (Cvtop t2 Reinterpret t1 sx) =>
-      if ves is v :: ves' then
-        if types_agree t1 v && (sx == None)
-        then ret (s, vs, RS_normal (vs_to_es (wasm_deserialise (bits v) t2 :: ves')))
-        else ret (s, vs, crash_error)
-      else ret (s, vs, crash_error)
-
-    (** control-flow instructions **)
-    | Basic Unreachable => ret (s, vs, RS_normal ((vs_to_es ves) ++ [::Trap]))
-    | Basic Nop => ret (s, vs, RS_normal (vs_to_es ves))
-    | Basic Drop =>
-      if ves is v :: ves' then
-        ret (s, vs, RS_normal (vs_to_es ves'))
-      else ret (s, vs, crash_error)
-    | Basic Select =>
-      if ves is (ConstInt32 c) :: v2 :: v1 :: ves' then
-        if c == Wasm_int.int_zero i32m
-        then ret (s, vs, RS_normal (vs_to_es (v2 :: ves')))
-        else ret (s, vs, RS_normal (vs_to_es (v1 :: ves')))
-      else ret (s, vs, crash_error)
-    | Basic (Block (Tf t1s t2s) es) =>
-      if length ves >= length t1s
+  (** convert and reinterpret **)
+  | Basic (Cvtop t2 Convert t1 sx) =>
+    if ves is v :: ves' then
+      if types_agree t1 v
       then
-        let: (ves', ves'')  := split_n ves (length t1s) in
-        ret (s, vs, RS_normal (vs_to_es ves''
-                              ++ [::Label (length t2s) [::] (vs_to_es ves' ++ to_e_list es)]))
+        expect (cvt t2 sx v) (fun v' =>
+             ret (s, vs, RS_normal (vs_to_es (v' :: ves'))))
+          (ret (s, vs, RS_normal ((vs_to_es ves') ++ [::Trap])))
       else ret (s, vs, crash_error)
-    | Basic (Loop (Tf t1s t2s) es) =>
-      if length ves >= length t1s
+    else ret (s, vs, crash_error)
+  | Basic (Cvtop t2 Reinterpret t1 sx) =>
+    if ves is v :: ves' then
+      if types_agree t1 v && (sx == None)
+      then ret (s, vs, RS_normal (vs_to_es (wasm_deserialise (bits v) t2 :: ves')))
+      else ret (s, vs, crash_error)
+    else ret (s, vs, crash_error)
+
+  (** control-flow instructions **)
+  | Basic Unreachable => ret (s, vs, RS_normal ((vs_to_es ves) ++ [::Trap]))
+  | Basic Nop => ret (s, vs, RS_normal (vs_to_es ves))
+  | Basic Drop =>
+    if ves is v :: ves' then
+      ret (s, vs, RS_normal (vs_to_es ves'))
+    else ret (s, vs, crash_error)
+  | Basic Select =>
+    if ves is (ConstInt32 c) :: v2 :: v1 :: ves' then
+      if c == Wasm_int.int_zero i32m
+      then ret (s, vs, RS_normal (vs_to_es (v2 :: ves')))
+      else ret (s, vs, RS_normal (vs_to_es (v1 :: ves')))
+    else ret (s, vs, crash_error)
+  | Basic (Block (Tf t1s t2s) es) =>
+    if length ves >= length t1s
+    then
+      let: (ves', ves'')  := split_n ves (length t1s) in
+      ret (s, vs, RS_normal (vs_to_es ves''
+                            ++ [::Label (length t2s) [::] (vs_to_es ves' ++ to_e_list es)]))
+    else ret (s, vs, crash_error)
+  | Basic (Loop (Tf t1s t2s) es) =>
+    if length ves >= length t1s
+    then
+      let: (ves', ves'') := split_n ves (length t1s) in
+      ret (s, vs, RS_normal (vs_to_es ves''
+                            ++ [::Label (length t1s) [::Basic (Loop (Tf t1s t2s) es)]
+                                    (vs_to_es ves' ++ to_e_list es)]))
+    else ret (s, vs, crash_error)
+  | Basic (If tf es1 es2) =>
+    if ves is ConstInt32 c :: ves' then
+      if c == Wasm_int.int_zero i32m
+      then ret (s, vs, RS_normal (vs_to_es ves' ++ [::Basic (Block tf es2)]))
+      else ret (s, vs, RS_normal (vs_to_es ves' ++ [::Basic (Block tf es1)]))
+    else ret (s, vs, crash_error)
+  | Basic (Br j) => ret (s, vs, RS_break j ves)
+  | Basic (Br_if j) =>
+    if ves is ConstInt32 c :: ves' then
+      if c == Wasm_int.int_zero i32m
+      then ret (s, vs, RS_normal (vs_to_es ves'))
+      else ret (s, vs, RS_normal (vs_to_es ves' ++ [::Basic (Br j)]))
+    else ret (s, vs, crash_error)
+  | Basic (Br_table js j) =>
+    if ves is ConstInt32 c :: ves' then
+      let: k := Wasm_int.nat_of_uint i32m c in
+      if k < length js
       then
-        let: (ves', ves'') := split_n ves (length t1s) in
-        ret (s, vs, RS_normal (vs_to_es ves''
-                              ++ [::Label (length t1s) [::Basic (Loop (Tf t1s t2s) es)]
-                                      (vs_to_es ves' ++ to_e_list es)]))
-      else ret (s, vs, crash_error)
-    | Basic (If tf es1 es2) =>
-      if ves is ConstInt32 c :: ves' then
-        if c == Wasm_int.int_zero i32m
-        then ret (s, vs, RS_normal (vs_to_es ves' ++ [::Basic (Block tf es2)]))
-        else ret (s, vs, RS_normal (vs_to_es ves' ++ [::Basic (Block tf es1)]))
-      else ret (s, vs, crash_error)
-    | Basic (Br j) => ret (s, vs, RS_break j ves)
-    | Basic (Br_if j) =>
-      if ves is ConstInt32 c :: ves' then
-        if c == Wasm_int.int_zero i32m
-        then ret (s, vs, RS_normal (vs_to_es ves'))
-        else ret (s, vs, RS_normal (vs_to_es ves' ++ [::Basic (Br j)]))
-      else ret (s, vs, crash_error)
-    | Basic (Br_table js j) =>
-      if ves is ConstInt32 c :: ves' then
-        let: k := Wasm_int.nat_of_uint i32m c in
-        if k < length js
-        then
-          ret (expect (List.nth_error js k) (fun js_at_k =>
-              (s, vs, RS_normal (vs_to_es ves' ++ [::Basic (Br js_at_k)])))
-            (s, vs, crash_error))
-        else ret (s, vs, RS_normal (vs_to_es ves' ++ [::Basic (Br j)]))
-      else ret (s, vs, crash_error)
-    | Basic (Call j) =>
-      if sfunc s i j is Some sfunc_i_j then
-        ret (s, vs, RS_normal (vs_to_es ves ++ [::Callcl sfunc_i_j]))
-      else ret (s, vs, crash_error)
-    | Basic (Call_indirect j) =>
-      if ves is ConstInt32 c :: ves' then
-        match stab s i (Wasm_int.nat_of_uint i32m c) with
-        | Some cl =>
-          if stypes s i j == Some (cl_type cl)
-          then ret (s, vs, RS_normal (vs_to_es ves' ++ [::Callcl cl]))
-          else ret (s, vs, RS_normal (vs_to_es ves' ++ [::Trap]))
-        | None => ret (s, vs, RS_normal (vs_to_es ves' ++ [::Trap]))
-        end
-      else ret (s, vs, crash_error)
-    | Basic Return => ret (s, vs, RS_return ves)
-    | Basic (Get_local j) =>
-      if j < length vs
-      then
-        ret (expect (List.nth_error vs j) (fun vs_at_j =>
-            (s, vs, RS_normal (vs_to_es (vs_at_j :: ves))))
+        ret (expect (List.nth_error js k) (fun js_at_k =>
+            (s, vs, RS_normal (vs_to_es ves' ++ [::Basic (Br js_at_k)])))
           (s, vs, crash_error))
+      else ret (s, vs, RS_normal (vs_to_es ves' ++ [::Basic (Br j)]))
+    else ret (s, vs, crash_error)
+  | Basic (Call j) =>
+    if sfunc s i j is Some sfunc_i_j then
+      ret (s, vs, RS_normal (vs_to_es ves ++ [::Callcl sfunc_i_j]))
+    else ret (s, vs, crash_error)
+  | Basic (Call_indirect j) =>
+    if ves is ConstInt32 c :: ves' then
+      match stab s i (Wasm_int.nat_of_uint i32m c) with
+      | Some cl =>
+        if stypes s i j == Some (cl_type cl)
+        then ret (s, vs, RS_normal (vs_to_es ves' ++ [::Callcl cl]))
+        else ret (s, vs, RS_normal (vs_to_es ves' ++ [::Trap]))
+      | None => ret (s, vs, RS_normal (vs_to_es ves' ++ [::Trap]))
+      end
+    else ret (s, vs, crash_error)
+  | Basic Return => ret (s, vs, RS_return ves)
+  | Basic (Get_local j) =>
+    if j < length vs
+    then
+      ret (expect (List.nth_error vs j) (fun vs_at_j =>
+          (s, vs, RS_normal (vs_to_es (vs_at_j :: ves))))
+        (s, vs, crash_error))
+    else ret (s, vs, crash_error)
+  | Basic (Set_local j) =>
+    if ves is v :: ves' then
+      if j < length vs
+      then ret (s, update_list_at vs j v, RS_normal (vs_to_es ves'))
       else ret (s, vs, crash_error)
-    | Basic (Set_local j) =>
-      if ves is v :: ves' then
-        if j < length vs
-        then ret (s, update_list_at vs j v, RS_normal (vs_to_es ves'))
-        else ret (s, vs, crash_error)
+    else ret (s, vs, crash_error)
+  | Basic (Tee_local j) =>
+    if ves is v :: ves' then
+      ret (s, vs, RS_normal (vs_to_es (v :: ves) ++ [::Basic (Set_local j)]))
+    else ret (s, vs, crash_error)
+  | Basic (Get_global j) =>
+    if sglob_val s i j is Some xx
+    then ret (s, vs, RS_normal (vs_to_es (xx :: ves)))
+    else ret (s, vs, crash_error)
+  | Basic (Set_global j) =>
+    if ves is v :: ves' then
+      if supdate_glob s i j v is Some xx
+      then ret (xx, vs, RS_normal (vs_to_es ves'))
       else ret (s, vs, crash_error)
-    | Basic (Tee_local j) =>
-      if ves is v :: ves' then
-        ret (s, vs, RS_normal (vs_to_es (v :: ves) ++ [::Basic (Set_local j)]))
-      else ret (s, vs, crash_error)
-    | Basic (Get_global j) =>
-      if sglob_val s i j is Some xx
-      then ret (s, vs, RS_normal (vs_to_es (xx :: ves)))
-      else ret (s, vs, crash_error)
-    | Basic (Set_global j) =>
-      if ves is v :: ves' then
-        if supdate_glob s i j v is Some xx
-        then ret (xx, vs, RS_normal (vs_to_es ves'))
-        else ret (s, vs, crash_error)
-      else ret (s, vs, crash_error)
-    | Basic (Load t None a off) =>
-      if ves is ConstInt32 k :: ves' then
-        expect
-          (smem_ind s i)
-          (fun j =>
-             if List.nth_error (s_memory s) j is Some mem_s_j then
-               expect
-                 (load (mem_s_j) (Wasm_int.nat_of_uint i32m k) off (t_length t))
-                 (fun bs =>
-                    ret (s, vs, RS_normal (vs_to_es (wasm_deserialise bs t :: ves'))))
-                 (ret (s, vs, RS_normal (vs_to_es ves' ++ [::Trap])))
-             else ret (s, vs, crash_error))
-          (ret (s, vs, crash_error))
-      else ret (s, vs, crash_error)
-    | Basic (Load t (Some (tp, sx)) a off) =>
-      if ves is ConstInt32 k :: ves' then
-        expect
-          (smem_ind s i)
-          (fun j =>
-             if List.nth_error (s_memory s) j is Some mem_s_j then
-               expect
-                 (load_packed sx (mem_s_j) (Wasm_int.nat_of_uint i32m k) off (tp_length tp) (t_length t))
-                 (fun bs =>
-                    ret (s, vs, RS_normal (vs_to_es (wasm_deserialise bs t :: ves'))))
-                 (ret (s, vs, RS_normal (vs_to_es ves' ++ [::Trap])))
-             else ret (s, vs, crash_error))
-          (ret (s, vs, crash_error))
-      else ret (s, vs, crash_error)
-    | Basic (Store t None a off) =>
-      if ves is v :: ConstInt32 k :: ves' then
-        if types_agree t v
-        then
-          expect
-            (smem_ind s i)
-            (fun j =>
-               if List.nth_error (s_memory s) j is Some mem_s_j then
-                 expect
-                   (store mem_s_j (Wasm_int.nat_of_uint i32m k) off (bits v) (t_length t))
-                   (fun mem' =>
-                      ret (upd_s_mem s (update_list_at (s_memory s) j mem'), vs, RS_normal (vs_to_es ves')))
-                   (ret (s, vs, RS_normal (vs_to_es ves' ++ [::Trap])))
-               else ret (s, vs, crash_error))
-            (ret (s, vs, crash_error))
-        else ret (s, vs, crash_error)
-      else ret (s, vs, crash_error)
-    | Basic (Store t (Some tp) a off) =>
-      if ves is v :: ConstInt32 k :: ves' then
-        if types_agree t v
-        then
-          expect
-            (smem_ind s i)
-            (fun j =>
-               if List.nth_error (s_memory s) j is Some mem_s_j then
-                 expect
-                   (store_packed mem_s_j (Wasm_int.nat_of_uint i32m k) off (bits v) (tp_length tp))
-                   (fun mem' =>
-                      ret (upd_s_mem s (update_list_at (s_memory s) j mem'), vs, RS_normal (vs_to_es ves')))
-                   (ret (s, vs, RS_normal (vs_to_es ves' ++ [::Trap])))
-               else ret (s, vs, crash_error))
-            (ret (s, vs, crash_error))
-        else ret (s, vs, crash_error)
-      else ret (s, vs, crash_error)
-    | Basic Current_memory =>
+    else ret (s, vs, crash_error)
+  | Basic (Load t None a off) =>
+    if ves is ConstInt32 k :: ves' then
       expect
         (smem_ind s i)
         (fun j =>
-           if List.nth_error (s_memory s) j is Some s_mem_s_j then
-             ret (s, vs, RS_normal (vs_to_es (ConstInt32 (Wasm_int.int_of_Z i32m (Z.of_nat (mem_size s_mem_s_j))) :: ves)))
+           if List.nth_error (s_memory s) j is Some mem_s_j then
+             expect
+               (load (mem_s_j) (Wasm_int.nat_of_uint i32m k) off (t_length t))
+               (fun bs =>
+                  ret (s, vs, RS_normal (vs_to_es (wasm_deserialise bs t :: ves'))))
+               (ret (s, vs, RS_normal (vs_to_es ves' ++ [::Trap])))
            else ret (s, vs, crash_error))
         (ret (s, vs, crash_error))
-    | Basic Grow_memory =>
-      if ves is ConstInt32 c :: ves' then
+    else ret (s, vs, crash_error)
+  | Basic (Load t (Some (tp, sx)) a off) =>
+    if ves is ConstInt32 k :: ves' then
+      expect
+        (smem_ind s i)
+        (fun j =>
+           if List.nth_error (s_memory s) j is Some mem_s_j then
+             expect
+               (load_packed sx (mem_s_j) (Wasm_int.nat_of_uint i32m k) off (tp_length tp) (t_length t))
+               (fun bs =>
+                  ret (s, vs, RS_normal (vs_to_es (wasm_deserialise bs t :: ves'))))
+               (ret (s, vs, RS_normal (vs_to_es ves' ++ [::Trap])))
+           else ret (s, vs, crash_error))
+        (ret (s, vs, crash_error))
+    else ret (s, vs, crash_error)
+  | Basic (Store t None a off) =>
+    if ves is v :: ConstInt32 k :: ves' then
+      if types_agree t v
+      then
         expect
           (smem_ind s i)
           (fun j =>
-            if List.nth_error (s_memory s) j is Some s_mem_s_j then
-              let: l := mem_size s_mem_s_j in
-              let: mem' := mem_grow s_mem_s_j (Wasm_int.nat_of_uint i32m c) in
-              let: s' := upd_s_mem s (update_list_at (s_memory s) j mem') in
-              ret (s', vs, RS_normal (vs_to_es (ConstInt32 (Wasm_int.int_of_Z i32m (Z.of_nat l)) :: ves')))
-            else ret (s, vs, crash_error))
+             if List.nth_error (s_memory s) j is Some mem_s_j then
+               expect
+                 (store mem_s_j (Wasm_int.nat_of_uint i32m k) off (bits v) (t_length t))
+                 (fun mem' =>
+                    ret (upd_s_mem s (update_list_at (s_memory s) j mem'), vs, RS_normal (vs_to_es ves')))
+                 (ret (s, vs, RS_normal (vs_to_es ves' ++ [::Trap])))
+             else ret (s, vs, crash_error))
           (ret (s, vs, crash_error))
       else ret (s, vs, crash_error)
-    | Basic (EConst _) => ret (s, vs, crash_error)
-    | Callcl cl =>
-      match cl with
-      | Func_native i' (Tf t1s t2s) ts es =>
-        let: n := length t1s in
-        let: m := length t2s in
-        if length ves >= n
-        then
-          let: (ves', ves'') := split_n ves n in
-          let: zs := n_zeros ts in
-          ret (s, vs, RS_normal (vs_to_es ves''
-                                ++ [::Local m i' (rev ves' ++ zs) [::Basic (Block (Tf [::] t2s) es)]]))
-        else ret (s, vs, crash_error)
-      | Func_host (Tf t1s t2s) f =>
-        let: n := length t1s in
-        let: m := length t2s in
-        if length ves >= n
-        then
-          let (ves', ves'') := split_n ves n in
-          r <- host_apply s f (rev ves') ;;
-          match r with
-          | Some (s', r) =>
-            (** We here double-check the types.
-              Note that this is not a requirement of the Wasm specification. **)
-            if result_types_agree t2s r
-            then
-              let: rves := result_to_stack r in
-              ret (s', vs, RS_normal (vs_to_es ves'' ++ rves))
-            else ret (s, vs, crash_error)
-          | None => ret (s, vs, crash_error) (* TODO *)
-          end
-        else ret (s, vs, crash_error)
-      end
-    | Label ln les es =>
-      if es_is_trap es
-      then ret (s, vs, RS_normal (vs_to_es ves ++ [::Trap]))
-      else
-        if const_list es
-        then ret (s, vs, RS_normal (vs_to_es ves ++ es))
-        else
-          rswf <- run_step_with_fuel fuel d i (s, vs, es) ;;
-          let: (s', vs', res) := rswf in
-          match res with
-          | RS_break 0 bvs =>
-            if length bvs >= ln
-            then ret (s', vs', RS_normal ((vs_to_es ((take ln bvs) ++ ves)) ++ les))
-            else ret (s', vs', crash_error)
-          | RS_break (n.+1) bvs => ret (s', vs', RS_break n bvs)
-          | RS_return rvs => ret (s', vs', RS_return rvs)
-          | RS_normal es' =>
-            ret (s', vs', RS_normal (vs_to_es ves ++ [::Label ln les es']))
-          | RS_crash error => ret (s', vs', RS_crash error)
-          end
-    | Local ln j vls es =>
-      if es_is_trap es
-      then ret (s, vs, RS_normal (vs_to_es ves ++ [::Trap]))
-      else
-        if const_list es
-        then
-          if length es == ln
-          then ret (s, vs, RS_normal (vs_to_es ves ++ es))
+    else ret (s, vs, crash_error)
+  | Basic (Store t (Some tp) a off) =>
+    if ves is v :: ConstInt32 k :: ves' then
+      if types_agree t v
+      then
+        expect
+          (smem_ind s i)
+          (fun j =>
+             if List.nth_error (s_memory s) j is Some mem_s_j then
+               expect
+                 (store_packed mem_s_j (Wasm_int.nat_of_uint i32m k) off (bits v) (tp_length tp))
+                 (fun mem' =>
+                    ret (upd_s_mem s (update_list_at (s_memory s) j mem'), vs, RS_normal (vs_to_es ves')))
+                 (ret (s, vs, RS_normal (vs_to_es ves' ++ [::Trap])))
+             else ret (s, vs, crash_error))
+          (ret (s, vs, crash_error))
+      else ret (s, vs, crash_error)
+    else ret (s, vs, crash_error)
+  | Basic Current_memory =>
+    expect
+      (smem_ind s i)
+      (fun j =>
+         if List.nth_error (s_memory s) j is Some s_mem_s_j then
+           ret (s, vs, RS_normal (vs_to_es (ConstInt32 (Wasm_int.int_of_Z i32m (Z.of_nat (mem_size s_mem_s_j))) :: ves)))
+         else ret (s, vs, crash_error))
+      (ret (s, vs, crash_error))
+  | Basic Grow_memory =>
+    if ves is ConstInt32 c :: ves' then
+      expect
+        (smem_ind s i)
+        (fun j =>
+          if List.nth_error (s_memory s) j is Some s_mem_s_j then
+            let: l := mem_size s_mem_s_j in
+            let: mem' := mem_grow s_mem_s_j (Wasm_int.nat_of_uint i32m c) in
+            let: s' := upd_s_mem s (update_list_at (s_memory s) j mem') in
+            ret (s', vs, RS_normal (vs_to_es (ConstInt32 (Wasm_int.int_of_Z i32m (Z.of_nat l)) :: ves')))
+          else ret (s, vs, crash_error))
+        (ret (s, vs, crash_error))
+    else ret (s, vs, crash_error)
+  | Basic (EConst _) => ret (s, vs, crash_error)
+  | Callcl cl =>
+    match cl with
+    | Func_native i' (Tf t1s t2s) ts es =>
+      let: n := length t1s in
+      let: m := length t2s in
+      if length ves >= n
+      then
+        let: (ves', ves'') := split_n ves n in
+        let: zs := n_zeros ts in
+        ret (s, vs, RS_normal (vs_to_es ves''
+                              ++ [::Local m i' (rev ves' ++ zs) [::Basic (Block (Tf [::] t2s) es)]]))
+      else ret (s, vs, crash_error)
+    | Func_host (Tf t1s t2s) f =>
+      let: n := length t1s in
+      let: m := length t2s in
+      if length ves >= n
+      then
+        let (ves', ves'') := split_n ves n in
+        r <- trigger (host_apply s f (rev ves')) ;;
+        match r with
+        | Some (s', r) =>
+          (** We here double-check the types.
+            Note that this is not a requirement of the Wasm specification. **)
+          if result_types_agree t2s r
+          then
+            let: rves := result_to_stack r in
+            ret (s', vs, RS_normal (vs_to_es ves'' ++ rves))
           else ret (s, vs, crash_error)
-        else
-          rswf <- run_step_with_fuel fuel d j (s, vls, es) ;;
-          let: (s', vls', res) := rswf in
-          match res with
-          | RS_return rvs =>
-            if length rvs >= ln
-            then ret (s', vs, RS_normal (vs_to_es (take ln rvs ++ ves)))
-            else ret (s', vs, crash_error)
-          | RS_normal es' =>
-            ret (s', vs, RS_normal (vs_to_es ves ++ [::Local ln j vls' es']))
-          | RS_crash error => ret (s', vs, RS_crash error)
-          | RS_break _ _ => ret (s', vs, crash_error)
-          end
-    | Trap => ret (s, vs, crash_error)
+        | None => ret (s, vs, crash_error) (* TODO *)
+        end
+      else ret (s, vs, crash_error)
     end
+  | Label ln les es =>
+    if es_is_trap es
+    then ret (s, vs, RS_normal (vs_to_es ves ++ [::Trap]))
+    else
+      if const_list es
+      then ret (s, vs, RS_normal (vs_to_es ves ++ es))
+      else
+        '(s', vs', res) <- call _ (call_run_step_base d i (s, vs, es)) ;;
+        match res with
+        | RS_break 0 bvs =>
+          if length bvs >= ln
+          then ret (s', vs', RS_normal ((vs_to_es ((take ln bvs) ++ ves)) ++ les))
+          else ret (s', vs', crash_error)
+        | RS_break (n.+1) bvs => ret (s', vs', RS_break n bvs)
+        | RS_return rvs => ret (s', vs', RS_return rvs)
+        | RS_normal es' =>
+          ret (s', vs', RS_normal (vs_to_es ves ++ [::Label ln les es']))
+        | RS_crash error => ret (s', vs', RS_crash error)
+        end
+  | Local ln j vls es =>
+    if es_is_trap es
+    then ret (s, vs, RS_normal (vs_to_es ves ++ [::Trap]))
+    else
+      if const_list es
+      then
+        if length es == ln
+        then ret (s, vs, RS_normal (vs_to_es ves ++ es))
+        else ret (s, vs, crash_error)
+      else
+        '(s', vls', res) <- call _ (call_run_step_base d j (s, vls, es)) ;;
+        match res return itree (run_stepE +' host_event) res_tuple with
+        | RS_return rvs =>
+          if length rvs >= ln
+          then ret (s', vs, RS_normal (vs_to_es (take ln rvs ++ ves)))
+          else ret (s', vs, crash_error)
+        | RS_normal es' =>
+          ret (s', vs, RS_normal (vs_to_es ves ++ [::Local ln j vls' es']))
+        | RS_crash error => ret (s', vs, RS_crash error)
+        | RS_break _ _ => ret (s', vs, crash_error)
+        end
+  | Trap => ret (s, vs, crash_error)
   end.
+
+Definition run_step_call : run_stepE ~> itree host_event :=
+  mrec (fun T (f : run_stepE T) =>
+    let call _ f := trigger f in
+    match f with
+    | call_run_step_base d i tt' =>
+      run_step_base call d i tt'
+    | call_run_one_step d i tt' e =>
+      run_one_step call d i tt' e
+    end).
 
 (** Enough fuel so that [run_one_step] does not run out of exhaustion. **)
 Definition run_one_step_fuel : administrative_instruction -> nat.
@@ -570,28 +580,25 @@ Definition run_step_fuel (tt : config_tuple) :=
   1 + List.fold_left max (List.map run_one_step_fuel es) 0.
 
 Definition run_step d j tt :=
-  run_step_with_fuel (run_step_fuel tt) d j tt.
+  burn (run_step_fuel tt) (run_step_call (call_run_step_base d j tt)).
 
-Fixpoint run_v (fuel : fuel) (d : depth) (i : instance) (tt : config_tuple)
-    : itree host_event (store_record * res) :=
-  let: (s, vs, es) := tt in
-  match fuel with
-  | 0 => ret (s, R_crash C_exhaustion)
-  | fuel.+1 =>
-    if es_is_trap es
-    then ret (s, R_trap)
-    else
-      if const_list es
-      then ret (s, R_value (fst (split_vals_e es)))
+Definition run_v : depth -> instance -> config_tuple -> itree host_event (store_record * res) :=
+  let run_v :=
+    rec-fix run_v (d, i, (s, vs, es)) :=
+      if es_is_trap es
+      then ret (s, R_trap) : 
+itree (callE (depth * instance * config_tuple) (store_record * res) +' host_event) (store_record * res)
       else
-        rs <- run_step d i (s, vs, es) ;;
-        let: (s', vs', res) := rs in
-        match res with
-        | RS_normal es' => run_v fuel d i (s', vs', es')
-        | RS_crash error => ret (s, R_crash error)
-        | _ => ret (s, R_crash C_error)
-        end
-  end.
+        if const_list es
+        then ret (s, R_value (fst (split_vals_e es)))
+        else
+          '(s', vs', r) <- run_step d i (s, vs, es) ;;
+          match r return itree (callE (depth * instance * config_tuple) (store_record * res) +' host_event) (store_record * res) with
+          | RS_normal es' => run_v (d, i, (s', vs', es'))
+          | RS_crash error => ret (s, R_crash error)
+          | _ => ret (s, R_crash C_error)
+          end in
+  fun d i tt => run_v (d, i, tt).
 
 End Host.
 
